theories/interpreter_ctx.v
@@ -1,0 +1,135 @@
+(** Proof-carrying interpreter for Wasm, optimised for contexts **)
+
+From Wasm Require Import common properties opsem_properties tactic typing_inversion contexts.
+From Coq Require Import ZArith.BinInt Program.Equality.
+From mathcomp Require Import ssreflect ssrfun ssrnat ssrbool eqtype seq.
+From Wasm Require Export operations host.
+Require Import BinNat.
+
+Set Implicit Arguments.
+Unset Strict Implicit.
+
+Unset Printing Implicit Defensive.
+
+Section Host.
+
+Import EvalContext.
+  
+Variable host_function : eqType.
+Let host := host host_function.
+Let cfg_tuple_ctx := @cfg_tuple_ctx host_function.
+
+Variable host_instance : host.
+
+Let store_record := store_record host_function.
+Let host_state := host_state host_instance.
+
+Let e_typing := @e_typing host_function.
+Let inst_typing := @inst_typing host_function.
+
+Variable host_application_impl : host_state -> store_record -> function_type -> host_function -> seq value ->
+                       (host_state * option (store_record * result)).
+
+Hypothesis host_application_impl_correct :
+  (forall hs s ft hf vs hs' hres, (host_application_impl hs s ft hf vs = (hs', hres)) -> host_application hs s ft hf vs hs' hres).
+
+Definition olist {T: Type} (ot: option T) : list T :=
+  match ot with
+  | Some t => [::t]
+  | None => nil
+  end.
+
+Definition reduce_cfg (hs hs': host_state) (cfg cfg': cfg_tuple_ctx) : Prop :=
+  match cfg with
+  | (s, f, cc, e) =>
+      match cfg' with
+      | (s', f', cc', e') => reduce hs s f (cc [[ olist e ]]) hs' s' f' (cc' [[ olist e' ]])
+      end
+  end.
+
+Definition run_one_step (hs: host_state) (cfg: cfg_tuple_ctx) : {hs' & {cfg' | reduce_cfg hs hs' cfg cfg'}}.
+Proof.
+  destruct cfg as [[[s f] cc] e].
+  destruct e as [e | ]; last first.
+Defined.
+
+End Host.
+
+Inductive res_crash : Type :=
+| C_error : res_crash
+| C_exhaustion : res_crash.
+
+Scheme Equality for res_crash.
+Definition res_crash_eqb c1 c2 := is_left (res_crash_eq_dec c1 c2).
+Definition eqres_crashP : Equality.axiom res_crash_eqb :=
+  eq_dec_Equality_axiom res_crash_eq_dec.
+
+Canonical Structure res_crash_eqMixin := EqMixin eqres_crashP.
+Canonical Structure res_crash_eqType := Eval hnf in EqType res_crash res_crash_eqMixin.
+
+Inductive res : Type :=
+| R_crash : res_crash -> res
+| R_trap : res
+| R_value : list value -> res.
+
+Definition res_eq_dec : forall r1 r2 : res, {r1 = r2} + {r1 <> r2}.
+Proof. decidable_equality. Defined.
+
+Definition res_eqb (r1 r2 : res) : bool := res_eq_dec r1 r2.
+Definition eqresP : Equality.axiom res_eqb :=
+  eq_dec_Equality_axiom res_eq_dec.
+
+Canonical Structure res_eqMixin := EqMixin eqresP.
+Canonical Structure res_eqType := Eval hnf in EqType res res_eqMixin.
+
+Section Host_func.
+
+Variable host_function : eqType.
+Let host := host host_function.
+
+Variable host_instance : host.
+
+Let store_record := store_record host_function.
+Let host_state := host_state host_instance.
+
+Let e_typing := @e_typing host_function.
+Let inst_typing := @inst_typing host_function.
+
+Variable host_application_impl : host_state -> store_record -> function_type -> host_function -> seq value ->
+                       (host_state * option (store_record * result)).
+
+Hypothesis host_application_impl_correct :
+  (forall hs s ft hf vs hs' hres, (host_application_impl hs s ft hf vs = (hs', hres)) -> host_application hs s ft hf vs hs' hres).
+
+(* Predicate for determining if a program fragment is typeable in some context, instead of a full program *)
+Definition fragment_typeable s f ves es :=
+  exists C C' ret lab t1s t2s t1s',
+    C = upd_label (upd_local_return C' (map typeof f.(f_locs)) ret) lab /\
+    rev [seq typeof i | i <- ves] = t1s' ++ t1s /\
+    inst_typing s f.(f_inst) C' /\
+    store_typing s /\
+    e_typing s C es (Tf t1s t2s).
+
+Inductive res_step'
+  (hs : host_state) (s : store_record) (f : frame)
+  (es : list administrative_instruction) : Type :=
+| RS'_value :
+    const_list es \/ es_is_trap es ->
+    res_step' hs s f es
+| RS'_error :
+    (~ fragment_typeable s f [::] es) ->
+    res_step' hs s f es
+| RS'_break k bvs :
+    (exists i j (lh: lholed i),
+      i + k = j /\
+      lfill lh (vs_to_es bvs ++ [::AI_basic (BI_br j)]) = es /\
+      empty_vs_base lh) ->
+    res_step' hs s f es
+| RS'_return rvs :
+    (exists i (lh: lholed i),
+      lfill lh (vs_to_es rvs ++ [:: AI_basic BI_return]) = es /\
+      empty_vs_base lh) ->
+    res_step' hs s f es
+| RS'_normal hs' s' f' es' :
+    reduce hs s f es hs' s' f' es' ->
+    res_step' hs s f es.
